lean/Ere.lean
@@ -1,0 +1,5 @@
+import Ere.Locale
+import Ere.Syntax
+import Ere.Semantics
+import Ere.Lemmas
+import Ere.Examples
